

Your Name:

Key

Calculus I, Math 151-11, Quiz #3

1. [5 points] Evaluate $\lim_{x \rightarrow \infty} \frac{3x - x^3}{x^2 + 14}$. Show all of your work. You may not use techniques that have not yet been introduced in this course.

$$\lim_{x \rightarrow \infty} \frac{3x - x^3}{x^2 + 14} \cdot \frac{1/x^2}{1/x^2} = \lim_{x \rightarrow \infty} \frac{\frac{3}{x} - x}{1 + \frac{14}{x^2}} = \frac{\frac{3}{\infty} - \infty}{1 + \frac{14}{\infty^2}} = \frac{0 - \infty}{1 + 0} = \frac{-\infty}{1+0} = \boxed{-\infty}$$

2. [10 points] Use the limit definition of a derivative to compute $f'(2)$ for $f(x) = \frac{x^2}{1+2x}$. (Hint: Compute $f'(2)$ directly, rather than computing $f'(x)$ and then plugging in $x=2$ at the end.)

$$\begin{aligned} f'(2) &= \lim_{h \rightarrow 0} \frac{f(2+h) - f(2)}{h} = \lim_{h \rightarrow 0} \frac{\frac{(2+h)^2}{1+2(2+h)} - \frac{4}{5}}{h} = \lim_{h \rightarrow 0} \frac{\frac{h^2 + 4h + 4}{5 + 2h} - \frac{4}{5}}{h} \\ &= \lim_{h \rightarrow 0} \frac{\frac{5h^2 + 20h + 20}{5(5+2h)} - \frac{4(5+2h)}{5(5+2h)}}{h} = \lim_{h \rightarrow 0} \frac{\frac{5h^2 + 20h + 20 - 20 - 8h}{25 + 10h}}{h} \\ &= \lim_{h \rightarrow 0} \frac{\frac{5h^2 + 12h}{25 + 10h}}{h/1} = \lim_{h \rightarrow 0} \frac{h(5h + 12)}{25 + 10h} \cdot \frac{1}{h} = \lim_{h \rightarrow 0} \frac{5h + 12}{25 + 10h} = \boxed{\frac{12}{25}} \end{aligned}$$

3. [10 points] Use the limit definition of the derivative to compute $g'(t)$, where $g(t) = \sqrt{3+4t}$.

$$\begin{aligned} g'(t) &= \lim_{h \rightarrow 0} \frac{g(t+h) - g(t)}{h} = \lim_{h \rightarrow 0} \frac{\sqrt{3+4(t+h)} - \sqrt{3+4t}}{h} = \lim_{t \rightarrow 0} \frac{\sqrt{3+4t+4h} - \sqrt{3+4t}}{h} \\ &= \lim_{t \rightarrow 0} \frac{(\sqrt{3+4t+4h} - \sqrt{3+4t})(\sqrt{3+4t+4h} + \sqrt{3+4t})}{h(\sqrt{3+4t+4h} + \sqrt{3+4t})} \\ &= \lim_{t \rightarrow 0} \frac{3+4t+4h - (3+4t)}{h(\sqrt{3+4t+4h} + \sqrt{3+4t})} = \lim_{h \rightarrow 0} \frac{4h}{h(\sqrt{3+4t+4h} + \sqrt{3+4t})} = \lim_{h \rightarrow 0} \frac{4}{\sqrt{3+4t+4h} + \sqrt{3+4t}} \\ &= \frac{4}{\sqrt{3+4t} + \sqrt{3+4t}} = \frac{4}{2\sqrt{3+4t}} = \boxed{\frac{2}{\sqrt{3+4t}}} \end{aligned}$$